git/yatima-inc/Megaparsec.lean/Megaparsec.lean
@@ -1,6 +1,3 @@
+import Megaparsec.ParserState
+import Megaparsec.Errors.Bundle
 import Megaparsec.Parsec
-import Megaparsec.RWST
-import Megaparsec.Stream
-import Megaparsec.Types
-import Megaparsec.Common
-import Megaparsec.MonadParsec
