git/yatima-inc/Megaparsec.lean/Megaparsec/Parsec.lean
@@ -1,32 +1,42 @@
-
-import Megaparsec.Types
+import Megaparsec.ParserState
 import Megaparsec.Stream
+import Megaparsec.Errors.StreamErrors
+import Megaparsec.Errors.StateErrors
 
 namespace Parsec
 
-/-- ParsecT data type and type class instances for it -/
+/-!
+Parsec transformer and abbreviation runners and relevant instances.
 
+Please find the most important functions for the users in the end of the file.
+-/
+
+/-- Parsec transformer, designed to add MonadParsec capability to any given monad M. -/
 structure ParsecT (E : Type) [stream : Stream.Stream S] [m : Monad M] (A : Type) where
+  -- TODO: Rewrite it as Lean 4 transformers (with `def`).
   unParser :
-    (B : Type) → (Types.State S E) →
+    (B : Type) → (ParserState.State S E) →
     -- Return A with State S E and Hints into M B
-    (A → Types.State S E → Errors.Hints (stream.Token) → M B) →    -- Consumed-OK
+    (A → ParserState.State S E → Errors.Hints (stream.Token) → M B) →          -- Consumed-OK
     -- Report errors with State into M B
-    (@Stream.ParseError S E stream → Types.State S E → M B) →      -- Consumed-Error
+    (@StreamErrors.ParseError S E stream → ParserState.State S E → M B) →      -- Consumed-Error
     -- Return A with State S E and Hints into M B
-    (A → Types.State S E → Errors.Hints (stream.Token) → M B) →    -- Empty-OK
+    (A → ParserState.State S E → Errors.Hints (stream.Token) → M B) →          -- Empty-OK
     -- Report errors with State into M B
-    (@Stream.ParseError S E stream → Types.State S E → M B) →      -- Empty-Error
+    (@StreamErrors.ParseError S E stream → ParserState.State S E → M B) →      -- Empty-Error
     M B
 
-def runParsecT (E : Type) [s : Stream.Stream S] 
-               [m : Monad M] (A : Type) 
-               (x : @ParsecT S M E s m A) (s₀: Types.State S E) : M (Types.Reply S E A) :=
+/-- Just add MonadParsec to Id. -/
+abbrev Parsec E S [stream : Stream.Stream S] := @ParsecT S Id E stream Id.instMonadId
+
+def runParsecT (E : Type) [s : Stream.Stream S]
+               [m : Monad M] (A : Type)
+               (x : @ParsecT S M E s m A) (s₀: ParserState.State S E) : M (ParserState.Reply S E A) :=
   let run_cok  := fun a s₁ _h => pure ⟨s₁, true,  .ok a⟩
   let run_cerr := fun err s₁  => pure ⟨s₁, true,  .err err⟩
   let run_eok  := fun a s₁ _h => pure ⟨s₁, false, .ok a⟩
   let run_eerr := fun err s₁  => pure ⟨s₁, false, .err err⟩
-  x.unParser (Types.Reply S E A) s₀ run_cok run_cerr run_eok run_eerr
+  x.unParser (ParserState.Reply S E A) s₀ run_cok run_cerr run_eok run_eerr
 
 def pPure [s : Stream.Stream S] [m : Monad M] (x : A) : @ParsecT S M E s m A :=
   ParsecT.mk $ fun b s _ _ eok _ => eok x s []
@@ -40,11 +50,11 @@ def pMap [s : Stream.Stream S] [m : Monad M] (f: U → V) (x : @ParsecT S M E s 
 instance [s : Stream.Stream S] [m : Monad M] : Functor (@ParsecT S M E s m) where
   map := pMap
 
-def pBind [s : Stream.Stream S] [m : Monad M] 
+def pBind [s : Stream.Stream S] [m : Monad M]
           (p : @ParsecT S M E s m A) (k : A → @ParsecT S M E s m B) : @ParsecT S M E s m B :=
   ParsecT.mk $ fun B s cok cerr eok eerr =>
-    let mcok x s' hs := ParsecT.unParser (k x) B s' cok cerr (Types.accHints hs cok) (Types.withHints hs cerr)
-    let meok x s' hs := ParsecT.unParser (k x) B s' cok cerr (Types.accHints hs eok) (Types.withHints hs eerr)
+    let mcok x s' hs := ParsecT.unParser (k x) B s' cok cerr (StateErrors.accHints hs cok) (StateErrors.withHints hs cerr)
+    let meok x s' hs := ParsecT.unParser (k x) B s' cok cerr (StateErrors.accHints hs eok) (StateErrors.withHints hs eerr)
     p.unParser B s mcok cerr meok eerr
 
 instance mprsₜ [s : Stream.Stream S] [m : Monad M] : Monad (@ParsecT S M E s m) where
@@ -52,20 +62,26 @@ instance mprsₜ [s : Stream.Stream S] [m : Monad M] : Monad (@ParsecT S M E s m
 
 /-- Alternative instance for ParsecT -/
 def pZero [s : Stream.Stream S] [m: Monad M] : @ParsecT S M E s m A :=
-  ParsecT.mk $ fun _ s _ _ _ eerr => eerr (Stream.ParseError.trivial s.stateOffset Option.none []) s
+  ParsecT.mk $ fun _ s _ _ _ eerr => eerr (StreamErrors.ParseError.trivial s.stateOffset Option.none []) s
 
 def pPlus [s : Stream.Stream S] [m : Monad M] [Ord (s.Token)] [BEq (Stream.Stream.Token S)]
           (p₁ : @ParsecT S M E s m A) (p₂ : @ParsecT S M E s m A) : @ParsecT S M E s m A :=
   ParsecT.mk $ fun B s cok cerr eok eerr =>
     let meer err ms :=
-        let ncerr err' s' := cerr (Stream.mergeError err' err) (Types.longestMatch ms s')
-        let neok x s' hs := eok x s' (Stream.toHints s'.stateOffset err ++ hs)
-        let neerr err' s' := eerr (Stream.mergeError err' err) (Types.longestMatch ms s')
+        let ncerr err' s' := cerr (StreamErrors.mergeError err' err) (ParserState.longestMatch ms s')
+        let neok x s' hs := eok x s' (StreamErrors.toHints s'.stateOffset err ++ hs)
+        let neerr err' s' := eerr (StreamErrors.mergeError err' err) (ParserState.longestMatch ms s')
         p₂.unParser B s cok ncerr neok neerr
     p₁.unParser B s cok cerr eok eerr
 
 instance altpₜ [s : Stream.Stream S] [Ord (s.Token)] [BEq (s.Token)] [m: Monad M] : Alternative (@ParsecT S M E s m) where
   failure := pZero
   orElse p₁ p₂ := pPlus p₁ (p₂ Unit.unit)
+
+--=========================================================--
+--================= IMPORTANT FUNCTIONS ===================--
+--=========================================================--
+
+-- def parse [Stream S] (Parsec E S A) String S : Util.Either ()
 
 end Parsec
